[pairing heaps] start next refinement function

Weidenbach_Book/IsaSAT/Pairing_Heaps_Impl.thy
@@ -31,6 +31,10 @@ lemma pairing_heaps_rel_def:
   unfolding pairing_heaps_rel_def_internal relAPP_def by auto
 
 
+definition op_hp_read_nxt_imp where
+  \<open>op_hp_read_nxt_imp = (\<lambda>i (prevs, nxts, children, parents, scores, h). do {
+      (nxts ! i)
+  })\<close>
 definition mop_hp_read_nxt_imp where
   \<open>mop_hp_read_nxt_imp = (\<lambda>i (prevs, nxts, children, parents, scores, h). do {
       ASSERT (i < length nxts);
@@ -51,6 +55,12 @@ lemma mop_hp_read_nxt_imp_spec:
     by (auto simp: pairing_heaps_rel_def map_fun_rel_def)
   done
 
+
+definition op_hp_read_prev_imp where
+  \<open>op_hp_read_prev_imp = (\<lambda>i (prevs, nxts, children, parents, scores, h). do {
+      prevs ! i
+  })\<close>
+
 definition mop_hp_read_prev_imp where
   \<open>mop_hp_read_prev_imp = (\<lambda>i (prevs, nxts, children, parents, scores, h). do {
       ASSERT (i < length prevs);
@@ -59,6 +69,12 @@ definition mop_hp_read_prev_imp where
 
 fun hp_read_prev' :: \<open>_\<close> where
   \<open>hp_read_prev' i (\<V>, arr, h) = hp_read_prev i arr\<close>
+
+lemma op_hp_read_prev_imp_spec:
+  \<open>(xs, ys) \<in> \<langle>R,S\<rangle>pairing_heaps_rel \<Longrightarrow> j \<in> fst ys \<Longrightarrow> (i,j)\<in>nat_rel \<Longrightarrow>
+  (op_hp_read_prev_imp i xs, hp_read_prev' j ys) \<in> R\<close>
+  unfolding op_hp_read_prev_imp_def
+  by (auto simp: pairing_heaps_rel_def map_fun_rel_def)
 
 lemma mop_hp_read_prev_imp_spec:
   \<open>(xs, ys) \<in> \<langle>R,S\<rangle>pairing_heaps_rel \<Longrightarrow> j \<in> fst ys \<Longrightarrow> (i,j)\<in>nat_rel \<Longrightarrow>
@@ -70,6 +86,11 @@ lemma mop_hp_read_prev_imp_spec:
   subgoal
     by (auto simp: pairing_heaps_rel_def map_fun_rel_def)
   done
+
+definition op_hp_read_child_imp where
+  \<open>op_hp_read_child_imp = (\<lambda>i (prevs, nxts, children, parents, scores, h). do {
+      (children ! i)
+  })\<close>
 
 definition mop_hp_read_child_imp where
   \<open>mop_hp_read_child_imp = (\<lambda>i (prevs, nxts, children, parents, scores, h). do {
@@ -96,10 +117,20 @@ definition mop_hp_read_parent_imp where
       ASSERT (i < length parents);
       RETURN (parents ! i)
   })\<close>
+definition op_hp_read_parent_imp where
+  \<open>op_hp_read_parent_imp = (\<lambda>i (prevs, nxts, children, parents, scores, h). do {
+      (parents ! i)
+  })\<close>
 
 fun hp_read_parent' :: \<open>_\<close> where
   \<open>hp_read_parent' i (\<V>, arr, h) = hp_read_parent i arr\<close>
 
+lemma op_hp_read_parent_imp_spec:
+  \<open>(xs, ys) \<in> \<langle>R,S\<rangle>pairing_heaps_rel \<Longrightarrow> j \<in> fst ys \<Longrightarrow> (i,j)\<in>nat_rel \<Longrightarrow>
+  (op_hp_read_parent_imp i xs, hp_read_parent' j ys) \<in> R\<close>
+  unfolding op_hp_read_parent_imp_def
+  by (auto simp: pairing_heaps_rel_def map_fun_rel_def)
+ 
 lemma mop_hp_read_parent_imp_spec:
   \<open>(xs, ys) \<in> \<langle>R,S\<rangle>pairing_heaps_rel \<Longrightarrow> j \<in> fst ys \<Longrightarrow> (i,j)\<in>nat_rel \<Longrightarrow>
   mop_hp_read_parent_imp i xs \<le> SPEC (\<lambda>a. (a, hp_read_parent' j ys) \<in> R)\<close>
@@ -111,7 +142,12 @@ lemma mop_hp_read_parent_imp_spec:
     by (auto simp: pairing_heaps_rel_def map_fun_rel_def)
   done
 
-definition mop_hp_read_score_imp where
+definition op_hp_read_score_imp :: \<open>nat \<Rightarrow> ('a,'b)pairing_heaps_imp \<Rightarrow> 'b\<close> where
+  \<open>op_hp_read_score_imp = (\<lambda>i (prevs, nxts, children, parents, scores, h). do {
+      ((scores ! i))
+  })\<close>
+
+definition mop_hp_read_score_imp :: \<open>nat \<Rightarrow> ('a,'b)pairing_heaps_imp \<Rightarrow> 'b nres\<close> where
   \<open>mop_hp_read_score_imp = (\<lambda>i (prevs, nxts, children, parents, scores, h). do {
       ASSERT (i < length scores);
       RETURN ((scores ! i))
@@ -167,7 +203,7 @@ fun source_node :: \<open>(nat set \<times> (nat,'c) hp_fun \<times> nat option)
 fun update_source_node_impl :: \<open>_ \<Rightarrow> ('a,'b)pairing_heaps_imp  \<Rightarrow> ('a,'b)pairing_heaps_imp\<close> where
   \<open>update_source_node_impl i (prevs, nxts, parents, children, scores,_) = (prevs, nxts, parents, children, scores, i)\<close>
 
-fun source_node_impl :: \<open>('a,'b)pairing_heaps_imp \<Rightarrow> _\<close> where
+fun source_node_impl :: \<open>('a,'b)pairing_heaps_imp \<Rightarrow> 'a option\<close> where
   \<open>source_node_impl (prevs, nxts, parents, children, scores,h) = h\<close>
 
 lemma update_source_node_impl_spec:
@@ -184,7 +220,7 @@ fun hp_update_parents' where
   \<open>hp_update_parents' i p(\<V>, u, h) = (\<V>, hp_update_parents i p u, h)\<close>
 
 fun hp_update_prev' where
-  \<open>hp_update_prev' i p(\<V>, u, h) = (\<V>, hp_update_prev i p u, h)\<close>
+  \<open>hp_update_prev' i p (\<V>, u, h) = (\<V>, hp_update_prev i p u, h)\<close>
 
 fun hp_update_nxt' where
   \<open>hp_update_nxt' i p(\<V>, u, h) = (\<V>, hp_update_nxt i p u, h)\<close>
@@ -197,7 +233,8 @@ lemma hp_insert_alt_def:
   let h = source_node arr;
   if h = None then do {
     ASSERT (i \<in> fst arr);
-    RETURN (update_source_node (Some i) (hp_set_all' i None None None None (Some w) arr))
+    let arr = (hp_set_all' i None None None None (Some w) arr);
+    RETURN (update_source_node (Some i) arr)
    } else do {
     ASSERT (i \<in> fst arr);
     ASSERT (hp_read_prev' i arr = None);
@@ -211,7 +248,6 @@ lemma hp_insert_alt_def:
     then do {
       let arr = hp_set_all' i None None (Some j) None (Some w) arr;
       let arr = hp_update_parents' j (Some i) arr;
-      let nxt = hp_read_nxt' j arr;
       RETURN (update_source_node (Some i) arr)
     }
     else do {
@@ -227,37 +263,97 @@ lemma hp_insert_alt_def:
    unfolding hp_insert_def
    by (auto intro!: ext bind_cong[OF refl] simp: Let_def)
 
-(*
-definition mop_hp_insert_impl :: \<open>'a \<Rightarrow> 'b::linorder \<Rightarrow> ('a,'b)pairing_heaps_imp \<Rightarrow> ('a,'b)pairing_heaps_imp nres\<close> where
-  \<open>mop_hp_insert_impl = (\<lambda>(i::'a) (w::'b) (\<V>::'a set, arr :: ('a, 'b) hp_fun, h :: 'a option). do {
+definition mop_hp_update_prev'_imp :: \<open>nat \<Rightarrow> 'a option \<Rightarrow> ('a,'b)pairing_heaps_imp \<Rightarrow> ('a,'b)pairing_heaps_imp nres\<close> where
+  \<open>mop_hp_update_prev'_imp = (\<lambda>i v (prevs, nxts, parents, children). do {
+    ASSERT (i < length prevs);
+    RETURN (prevs[i:=v], nxts, parents, children)
+  })\<close>
+
+
+lemma mop_hp_update_prev'_imp_spec:
+  \<open>(xs, ys) \<in> \<langle>R,S\<rangle>pairing_heaps_rel \<Longrightarrow> j \<in> fst ys \<Longrightarrow> (i,j)\<in>nat_rel \<Longrightarrow>
+   (p',p)\<in>R \<Longrightarrow>
+  mop_hp_update_prev'_imp i p' xs \<le> SPEC (\<lambda>a. (a, hp_update_prev' j p ys) \<in> \<langle>R,S\<rangle>pairing_heaps_rel)\<close>
+  unfolding mop_hp_update_prev'_imp_def
+  apply refine_vcg
+  subgoal
+    by (auto simp: pairing_heaps_rel_def map_fun_rel_def hp_update_prev_def)
+  subgoal
+    by (force simp: pairing_heaps_rel_def map_fun_rel_def hp_update_prev_def)
+  done
+
+definition mop_hp_update_parent'_imp :: \<open>nat \<Rightarrow> 'a option \<Rightarrow> ('a,'b)pairing_heaps_imp \<Rightarrow> ('a,'b)pairing_heaps_imp nres\<close> where
+  \<open>mop_hp_update_parent'_imp = (\<lambda>i v (prevs, nxts,children, parents, scores). do {
+    ASSERT (i < length parents);
+    RETURN (prevs, nxts, children, parents[i:=v], scores)
+  })\<close>
+
+
+lemma mop_hp_update_parent'_imp_spec:
+  \<open>(xs, ys) \<in> \<langle>R,S\<rangle>pairing_heaps_rel \<Longrightarrow> j \<in> fst ys \<Longrightarrow> (i,j)\<in>nat_rel \<Longrightarrow>
+   (p',p)\<in>R \<Longrightarrow>
+  mop_hp_update_parent'_imp i p' xs \<le> SPEC (\<lambda>a. (a, hp_update_parents' j p ys) \<in> \<langle>R,S\<rangle>pairing_heaps_rel)\<close>
+  unfolding mop_hp_update_parent'_imp_def
+  apply refine_vcg
+  subgoal
+    by (auto simp: pairing_heaps_rel_def map_fun_rel_def hp_update_parents_def)
+  subgoal
+    by (force simp: pairing_heaps_rel_def map_fun_rel_def hp_update_parents_def)
+  done
+
+(*TODO it is kind of unclear whether we should use nat or have a conversion 'a \<Rightarrow> nat as locale*)
+definition mop_hp_insert_impl :: \<open>nat \<Rightarrow> 'b::linorder \<Rightarrow> (nat,'b)pairing_heaps_imp \<Rightarrow> (nat,'b)pairing_heaps_imp nres\<close> where
+  \<open>mop_hp_insert_impl = (\<lambda>i (w::'b) (arr :: (nat,'b)pairing_heaps_imp). do {
+  let h = source_node_impl arr;
   if h = None then do {
-    ASSERT (i \<in> \<V>);
-    RETURN (\<V>, hp_set_all i None None None None (Some w) arr, Some i)
+    arr \<leftarrow> mop_hp_set_all_imp i None None None None w arr;
+    RETURN (update_source_node_impl (Some i) arr)
    } else do {
-    ASSERT (i \<in> \<V>);
-    ASSERT (hp_read_prev i arr = None);
-    ASSERT (hp_read_parent i arr = None);
-    let (j::'a) = ((the h) :: 'a);
-    ASSERT (j \<in> (\<V>::'a set) \<and> j \<noteq> i);
-    ASSERT (hp_read_score j (arr :: ('a, 'b) hp_fun) \<noteq> None);
-    ASSERT (hp_read_prev j arr = None \<and> hp_read_nxt j arr = None \<and> hp_read_parent j arr = None);
-    let y = (the (hp_read_score j arr)::'b);
+    ASSERT (op_hp_read_prev_imp i arr = None);
+    ASSERT (op_hp_read_parent_imp i arr = None);
+    let j = (the h);
+    ASSERT (op_hp_read_prev_imp j arr = None \<and> op_hp_read_nxt_imp j arr = None \<and> op_hp_read_parent_imp j arr = None);
+    y \<leftarrow> mop_hp_read_score_imp j arr;
     if y < w
     then do {
-      let arr = hp_set_all i None None (Some j) None (Some (w::'b)) (arr::('a, 'b) hp_fun);
-      let arr = hp_update_parents j (Some i) arr;
-      let nxt = hp_read_nxt j arr;
-      RETURN (\<V>, arr :: ('a, 'b) hp_fun, Some i)
+      arr \<leftarrow> mop_hp_set_all_imp i None None (Some j) None ((w)) (arr);
+      arr\<leftarrow> mop_hp_update_parent'_imp j (Some i) arr;
+      RETURN (update_source_node_impl (Some i) arr)
     }
     else do {
-      let child = hp_read_child j arr;
-      let arr = hp_set_all j None None (Some i) None (Some y) arr;
-      let arr = hp_set_all i None child None (Some j) (Some (w::'b)) arr;
-      let arr = (if child = None then arr else hp_update_prev (the child) (Some i) arr);
-      let arr = (if child = None then arr else hp_update_parents (the child) None arr);
-      RETURN (\<V>, arr :: ('a, 'b) hp_fun, h)
+      let child = op_hp_read_child_imp j arr;
+      arr \<leftarrow> mop_hp_set_all_imp j None None (Some i) None (y) arr;
+      arr \<leftarrow> mop_hp_set_all_imp i None child None (Some j) w arr;
+      arr \<leftarrow> (if child = None then RETURN arr else mop_hp_update_prev'_imp (the child) (Some i) arr);
+      arr \<leftarrow> (if child = None then RETURN arr else mop_hp_update_parent'_imp (the child) None arr);
+      RETURN arr
     }
    }
   })\<close>
-*)
+
+lemma
+  \<open>(xs, ys) \<in> \<langle>\<langle>nat_rel\<rangle>option_rel,\<langle>S\<rangle>option_rel\<rangle>pairing_heaps_rel \<Longrightarrow> (i,j)\<in>nat_rel \<Longrightarrow> (w,w')\<in>S \<Longrightarrow>
+  mop_hp_insert_impl i w xs \<le> \<Down>(\<langle>\<langle>nat_rel\<rangle>option_rel,\<langle>S\<rangle>option_rel\<rangle>pairing_heaps_rel) (hp_insert j w' ys)\<close>
+  unfolding mop_hp_insert_impl_def hp_insert_alt_def
+  apply (refine_vcg mop_hp_set_all_imp_spec[where R=\<open>\<langle>nat_rel\<rangle>option_rel\<close> and S=\<open>\<langle>S\<rangle>option_rel\<close>])
+  subgoal by (auto dest: source_node_spec)
+  subgoal by auto
+  subgoal by auto
+  subgoal by auto
+  subgoal by auto
+  subgoal by auto
+  subgoal by (auto intro!: update_source_node_impl_spec simp: refl_on_def)
+  subgoal by (auto dest!: op_hp_read_prev_imp_spec)
+  subgoal by (auto dest!: op_hp_read_parent_imp_spec)
+  subgoal
+    using op_hp_read_parent_imp_spec[of xs ys \<open>\<langle>nat_rel\<rangle>option_rel\<close> \<open>\<langle>S\<rangle>option_rel\<close> \<open>the (source_node ys)\<close> \<open>the (source_node_impl xs)\<close>]
+      source_node_spec[of xs ys  \<open>\<langle>nat_rel\<rangle>option_rel\<close> \<open>\<langle>S\<rangle>option_rel\<close>]
+    by (metis op_hp_read_prev_imp_spec option_rel_simp(2) the_paramL)
+  subgoal
+    using op_hp_read_parent_imp_spec[of xs ys \<open>\<langle>nat_rel\<rangle>option_rel\<close> \<open>\<langle>S\<rangle>option_rel\<close> \<open>the (source_node ys)\<close> \<open>the (source_node_impl xs)\<close>]
+      source_node_spec[of xs ys  \<open>\<langle>nat_rel\<rangle>option_rel\<close> \<open>\<langle>S\<rangle>option_rel\<close>]
+    apply auto
+oops
+
+
 end
